\newpage
\section{矩阵的性质总结}
\subsection{转置}
\pro{转置的性质总结}{转置的性质总结}{
    $\bm{A}$、$\bm{B}$均为$n$阶方阵,$c \in \bb{R}$
    \begin{enumerate}[label=\arabic*)]
        \item $\left(\bm{A}^{\prime}\right)^{\prime} = \bm{A}$
        \item $\left(\bm{AB}\right)^{\prime} =
                  \bm{B}^{\prime}\bm{A}^{\prime} $
        \item $\left(c\bm{A}\right)^{\prime} = c\bm{A}^{\prime}$
        \item $\left|\bm{A}^{\prime}\right|
                  =\left|\bm{A}\right|$
    \end{enumerate}
}
\subsection{逆阵}
\pro{逆阵的性质总结}{逆阵的性质总结}{
    $\bm{A}$、$\bm{B}$均为$n$阶可逆方阵$\left(
        \left|\bm{A}\right|
        =\left|\bm{B}\right|
        \neq 0
        \right)$,$c \in \bb{R}$
    \begin{enumerate}[label=\arabic*)]
        \item 逆阵存在则唯一
        \item $ \left(\bm{A}^{-1}\right)^{-1}
                  = \bm{A} $
        \item $\left(\bm{AB}\right)^{-1}
                  = \bm{B}^{-1}\bm{A}^{-1}$
        \item$\left(c\bm{A}\right)^{-1}
                  =c^{-1}\bm{A}^{-1}$
        \item $\left|\bm{A}^{-1}\right|
                  = \left|\bm{A}\right|^{-1}$
        \item $\left(\bm{A}^{\prime}\right)^{-1}
                  = \left(\bm{A}^{-1}\right)^{\prime}$
        \item 整性对可逆阵成立
        \item 消去律对可逆阵成立
    \end{enumerate}
}
\subsection{伴随阵}
\pro{伴随阵的性质总结}{伴随阵的性质总结}{
    $\bm{A}$、$\bm{B}$均为$n$阶方阵,$c \in \bb{R}$,$n \geqslant 2$
    \begin{enumerate}[label=\textup{(\arabic*)}]
        \item 伴随阵必定存在
        \item $\bm{AA}^* = \bm{A}^*\bm{A}
                  = \left|\bm{A}\right|\bm{I}_n$
        \item  $\left(\bm{A}^*\right)^*=
                  \begin{cases*}
                      \left|\bm{A}\right|
                      ^{n - 2}\bm{A},n\geqslant 3 \\
                      \bm{A},n = 2
                  \end{cases*}$
        \item $\left(\bm{AB}\right)^* =
                  \bm{B}^*\bm{A}^*$
        \item $\left(c\bm{A}\right)^*=
                  c^{n - 1}\bm{A}^*$
        \item $\left|\bm{A}^*\right|
                  =\left|\bm{A}\right|^{n - 1}$
        \item $\left(\bm{A}^{\prime}\right)^*
                  = \left(\bm{A}^*\right)^{\prime}$
        \item $\left|\bm{A}\right| \neq 0$
              时
              ,$\left(\bm{A}^{-1}\right)^*
                  =\left(\bm{A}^*\right)^{-1}$
        \item $\begin{pmatrix}
                      \bm{I}_r & \bm{O} \\
                      \bm{O}   & \bm{O}
                  \end{pmatrix}
                  ^* = \begin{cases*}
                      \bm{O},r \leqslant n - 2
                      \\
                      \begin{pmatrix}
                          \bm{O} & \bm{O} \\
                          0      & 1
                      \end{pmatrix},
                      r = n -1
                      \\
                      \bm{I}_n,
                      r = n
                  \end{cases*}\quad
                  \left(0 \leqslant r
                  \leqslant n\right)
              $
        \item $r < n$时
              $\displaystyle
                  \left|\begin{pmatrix}
                      \bm{I}_r & \bm{O} \\
                      \bm{O}   & \bm{O}
                  \end{pmatrix}
                  ^*\right|=0
              $
        \item $\displaystyle
                  \left(
                  \begin{pmatrix}
                      \bm{I}_r & \bm{O} \\
                      \bm{O}   & \bm{O}
                  \end{pmatrix}
                  ^*
                  \right)^*=\begin{cases*}
                      \begin{pmatrix}
                          \bm{I}_r & \bm{O} \\
                          \bm{O}   & \bm{O}
                      \end{pmatrix},n=2,r=1 \\
                      \bm{I}_n,r=n          \\
                      \bm{O},\text{其他}
                  \end{cases*}
              $
    \end{enumerate}
}